eve/Src/Eiffel/interface/graphical/tools/autoproof/es_autoproof_bench_helper.e
@@ -1,6 +1,6 @@
 note
 	description: "[
-		TODO
+		Helper class to minimize changes of proper EiffelStudio for the integration of AutoProof.
 	]"
 	date: "$Date$"
 	revision: "$Revision$"
@@ -89,7 +89,7 @@ feature -- Verification
 		end
 
 note
-	copyright: "Copyright (c) 1984-2012, Eiffel Software"
+	copyright: "Copyright (c) 1984-2013, Eiffel Software"
 	license: "GPL version 2 (see http://www.eiffel.com/licensing/gpl.txt)"
 	licensing_options: "http://www.eiffel.com/licensing"
 	copying: "[
