eve/Src/framework/eiffel2boogie/iv/iv_generic_type.e
@@ -37,4 +37,12 @@ feature -- Visitor
 			a_visitor.process_generic_type (Current)
 		end
 
+feature -- Equality
+
+	is_same_type (a_other: IV_TYPE): BOOLEAN
+			-- Is `a_other' same type as this?
+		do
+			Result := True
+		end
+
 end
